proved types equiv is a partial equivalence relations

theories/AlmostStlc/Types.v
@@ -1,3 +1,5 @@
+From Equations Require Import Equations Signature.
+
 Inductive type : Type :=
   | Nat : type
   | List : type -> type
@@ -9,3 +11,40 @@ Notation call_frame := (list (type * type)).
 Notation mfix_ctx := (list call_frame).
 
 Notation vtype := type.
+
+
+Section type_mutind.
+
+  Context (Pt : type -> Prop) (Pmfix : mfix_ctx -> Prop) (Pcall : call_frame -> Prop).
+
+  Context (HNat : Pt Nat).
+  Context (HList : forall t : type, Pt t -> Pt (List t)).
+  Context (HPair : forall t1 t2, Pt t1 -> Pt t2 -> Pt (Pair t1 t2)).
+  Context (HArrow : forall t1 MR t2, Pt t1 -> Pmfix MR -> Pt t2 -> Pt (Arrow t1 MR t2)).
+  Context (Hnil1 : Pmfix nil) (Hcons1 : forall R MR, Pcall R -> Pmfix MR -> Pmfix (cons R MR)).
+  Context (Hnil2 : Pcall nil) (Hcons2 : forall t1 t2 R, Pt t1 -> Pt t2 -> Pcall R -> Pcall (cons (t1, t2) R)).
+  
+  Equations type_mutind (t : type) : Pt t :=
+    {
+      type_mutind Nat := HNat;
+      type_mutind (List t) := HList t (type_mutind t);
+      type_mutind (Pair t1 t2) := HPair t1 t2 (type_mutind t1) (type_mutind t2);
+      type_mutind (Arrow t1 MR t2) := HArrow t1 MR t2 (type_mutind t1) (mfix_mutind MR) (type_mutind t2);
+    }
+   where mfix_mutind (MR : mfix_ctx) : Pmfix MR :=
+     {
+       mfix_mutind nil := Hnil1;
+       mfix_mutind (cons R MR) := Hcons1 R MR (call_frame_mutind R) (mfix_mutind MR);
+     }
+   where call_frame_mutind (R : call_frame) : Pcall R :=
+     {
+       call_frame_mutind nil := Hnil2;
+       call_frame_mutind (cons (t1,t2) R) := Hcons2 t1 t2 R (type_mutind t1) (type_mutind t2) (call_frame_mutind R);
+     }.
+
+  Theorem type_mfix_mutind : (forall t, Pt t) /\ (forall MR, Pmfix MR) /\ (forall R, Pcall R).
+  Proof.
+    repeat split; try apply type_mutind; try apply mfix_mutind; try apply call_frame_mutind.
+  Qed.
+
+End type_mutind.
