theories/AlmostStlc/TypesEquiv.v
@@ -16,9 +16,25 @@ Require Import ExtLib.Structures.Monad.
 Import MonadNotation.
 Local Open Scope monad_scope.
 
+From Coq Require Import
+     Program
+     Setoid
+     Morphisms
+     RelationClasses.
+
+
 Inductive list_rel {A} (R : Rel A A): Rel (list A) (list A) :=
   | list_rel_nil : list_rel R nil nil
   | list_rel_cons a b l1 l2 : R a b ->list_rel R l1 l2 -> list_rel R (cons a l1) (cons a l2).
+
+Theorem transitive_list_rel A (R : Rel A A) : Transitive R -> Transitive (list_rel R).
+Proof.
+  intros HTrans l1 l2 l3. revert l1 l3. induction l2.
+  - intros l1 l3 Hl12 Hl23. inversion Hl12. inversion Hl23. constructor.
+  - intros l1 l3 Hl12 Hl23. inversion Hl12. subst. inversion Hl23. subst.
+    econstructor; eauto.
+Qed.
+
 
 Equations types_equiv (t : type) : Rel (denote_type t) (denote_type t) := {
     types_equiv Nat := eq;
@@ -66,6 +82,11 @@ Fixpoint ctx_equiv (Γ : ctx) : Rel (denote_ctx Γ) (denote_ctx Γ) :=
 Definition comp_equiv {t Γ MR} :=
     fun c1 c2 => forall hyps1 hyps2, ctx_equiv Γ hyps1 hyps2 ->
               rutt (mfix_pre_equiv MR) (mfix_post_equiv MR) (types_equiv t) (c1 hyps1) (c2 hyps2).
+
+Definition mfix_bodies_equiv {Γ MR R} :=
+  fun bodies1 bodies2 => forall hyps1 hyps2 arg1 arg2, 
+      ctx_equiv Γ hyps1 hyps2 -> call_frame_pre_equiv R arg1 arg2 ->
+       rutt (mfix_pre_equiv MR) (mfix_post_equiv MR) (call_frame_post_equiv R arg1 arg2)  (bodies1 hyps1 arg1) (bodies2 hyps2 arg2).
 
 Lemma mfix_pre_call_mrec:
     forall (t1 t2 : vtype) (MR : mfix_ctx) (R : call_frame) (xR : var R MR) 
@@ -200,3 +221,73 @@ Proof.
   rewrite mfix_post_equiv_equation_2.
   intros. reflexivity.
 Qed.
+
+Lemma types_equiv_sym_prod : (forall t, Symmetric (types_equiv t)) /\ 
+                          (forall MR, Symmetric (mfix_pre_equiv MR) /\ SymmetricPostRel (mfix_post_equiv MR) ) /\
+                          (forall R, Symmetric (call_frame_pre_equiv R) /\ SymmetricPostRel (call_frame_post_equiv R)).
+Proof.
+  eapply type_mfix_mutind; intros; simp types_equiv.
+  - auto.
+  - intros l1 l2 Hl. induction Hl. constructor. econstructor; eauto.
+  - repeat intro. destruct H1. constructor; auto.
+  - intros f g Hfg x y Hxy. destruct H0. apply rutt_sym; auto.
+  - split; repeat intro; contradiction.
+  - destruct H. destruct H0. split.
+    + repeat intro. inversion H3; constructor; auto.
+    + repeat intro. dependent destruction H3; constructor; auto.
+  - cbn. split; repeat intro; contradiction.
+  - destruct H1. split; repeat intro.
+    + dependent destruction H3; constructor; auto.
+    + dependent destruction H3; constructor; auto.
+Qed.
+
+#[global] Instance types_equiv_sym : forall t : type, Symmetric (types_equiv t).
+Proof.
+  destruct types_equiv_sym_prod; auto.
+Qed.
+
+Lemma types_equiv_trans_prod : (forall t, Transitive (types_equiv t)) /\ 
+                          (forall MR, Transitive (mfix_pre_equiv MR) /\ TransitivePostRel (mfix_pre_equiv MR) (mfix_post_equiv MR) ) /\
+                          (forall R, Transitive (call_frame_pre_equiv R) /\ 
+                                  TransitivePostRel (call_frame_pre_equiv R) (call_frame_post_equiv R)).
+Proof.
+  eapply type_mfix_mutind; intros; simp types_equiv.
+  - repeat intro; subst; auto.
+  - apply transitive_list_rel. auto. 
+  - repeat intro. dependent destruction H1. dependent destruction H2.
+    constructor; eauto.
+  - intros f g h Hfg Hgh x y Hxy.
+    destruct H0.
+    eapply rutt_trans'; eauto.
+    apply Hgh. transitivity x; auto. symmetry. auto.
+  - split; repeat intro; contradiction.
+  - destruct H. destruct H0. split; repeat intro.
+    + dependent destruction H3; dependent destruction H4; constructor; eauto.
+    + dependent destruction H4; dependent destruction H5; dependent destruction H3.
+      * eapply H1 in H3; eauto. specialize (H3 a2 H4 H5). destruct H3 as [b [Hb1 Hb2] ].
+           exists b. split; constructor; auto.
+      * eapply H2 in H3; eauto. specialize (H3 b2 H4 H5). destruct H3 as [b [Hb1 Hb2]].
+           exists b. split; constructor; auto.
+  - split; repeat intro; contradiction.
+  - destruct H1. split; repeat intro.
+    + dependent destruction H3; dependent destruction H4; constructor; auto; etransitivity; eauto.
+    + dependent destruction H4; dependent destruction H5; dependent destruction H3.
+      * exists c. split; constructor; auto. transitivity a; eauto. symmetry. auto.
+      * eapply H2 in H3; eauto. specialize (H3 b2 H4 H5). destruct H3 as [b [Hb1 Hb2]].
+        exists b. split; constructor; eauto.
+Qed.
+
+#[global] Instance types_equiv_trans : forall t : type, Transitive (types_equiv t).
+Proof.
+  destruct types_equiv_trans_prod. auto.
+Qed.
+
+(*
+Lemma types_equiv_comp_refl_prop : 
+  (forall t Γ MR (c : comp t Γ MR), comp_equiv (denote_comp c) (denote_comp c)) /\
+  (forall t Γ (v : value t Γ), forall MR, comp_equiv (MR := MR) (denote_value v) (denote_value v)) /\
+    (* maybe I should look carefully at mfix_bodies type signature, maybe I can change it and get better results*)
+    (forall Γ MR' R (bodies : mfix_bodies Γ MR' R) MR, MR' = R :: MR -> mfix_bodies_equiv (denote_bodies bodies) (denote_bodies bodies)).
+Proof.
+  apply comp_value_mutind.
+*)
